semantics/replScript.sml
@@ -10,14 +10,14 @@ val _ = Hol_datatype `
 repl_state = <| (* Elaborator state *)
                 type_bindings : tdef_env; ctors : ctor_env;
                 (* Type system state *)
-                tenvM : tenvM; tenvC : tenvC; tenv : tenvE;
+                tdecs : tid_or_exn set; tenvM : tenvM; tenvC : tenvC; tenv : tenvE;
                 (* Semantics state *)
-                envM : envM; envC : envC; store : v store; envE : envE |>`;
+                envM : envM; envC : envC; store : (v store # tid_or_exn set); envE : envE |>`;
 
 val init_repl_state_def = Define`
   init_repl_state = <| type_bindings := init_type_bindings; ctors := [];
-                       tenvM := []; tenvC := init_tenvC; tenv := init_tenv;
-                       envM := []; envC := init_envC; store := []; envE := init_env |>`
+                       tdecs := {}; tenvM := []; tenvC := init_tenvC; tenv := init_tenv;
+                       envM := []; envC := init_envC; store := ([],{}); envE := init_env |>`
 
 val _ = Hol_datatype `
 repl_result =
@@ -30,11 +30,12 @@ strip_mod_env tenvM =
   MAP (\(n,tenv). (n,[])) tenvM`;
 
 val update_repl_state_def = Define `
-update_repl_state ast state type_bindings ctors tenvM tenvC tenv store envC r =
+update_repl_state ast state type_bindings ctors tdecs tenvM tenvC tenv store envC r =
   case r of
     | Rval (envM,envE) =>
         <| type_bindings := type_bindings ++ state.type_bindings;
            ctors := ctors ++ state.ctors;
+           tdecs := tdecs;
            tenvM := tenvM ++ state.tenvM;
            tenvC := merge_tenvC tenvC state.tenvC;
            tenv := bind_var_list2 tenv state.tenv;
@@ -124,19 +125,19 @@ val (ast_repl_rules, ast_repl_ind, ast_repl_cases) = Hol_reln `
 (!state.
   ast_repl state [] [] Terminate) ∧
 
-(!state type_errors ast asts top rest type_bindings' ctors' tenvM' tenvC' tenv' store' envC' r.
+(!state type_errors ast asts top rest type_bindings' ctors' tdecs' tenvM' tenvC' tenv' store' envC' r.
   (elab_top state.type_bindings state.ctors ast =
    (type_bindings', ctors', top)) ∧
-  (type_top state.tenvM state.tenvC state.tenv top tenvM' tenvC' tenv') ∧
+  (type_top state.tdecs state.tenvM state.tenvC state.tenv top tdecs' tenvM' tenvC' tenv') ∧
   evaluate_top (state.envM, state.envC, state.envE) state.store top (store',envC',r) ∧
-  ast_repl (update_repl_state top state type_bindings' ctors' tenvM' tenvC' tenv' store' envC' r) type_errors asts rest
+  ast_repl (update_repl_state top state type_bindings' ctors' tdecs' tenvM' tenvC' tenv' store' envC' r) type_errors asts rest
   ⇒
   ast_repl state (F::type_errors) (SOME ast::asts) (Result (print_result (tenv_to_string_map tenv') top envC' r) rest)) ∧
 
-(!state type_errors ast asts top type_bindings' ctors' tenvM' tenvC' tenv'.
+(!state type_errors ast asts top type_bindings' ctors' tdecs' tenvM' tenvC' tenv'.
   (elab_top state.type_bindings state.ctors ast =
    (type_bindings', ctors', top)) ∧
-  (type_top state.tenvM state.tenvC state.tenv top tenvM' tenvC' tenv') ∧
+  (type_top state.tdecs state.tenvM state.tenvC state.tenv top tdecs' tenvM' tenvC' tenv') ∧
   top_diverges (state.envM, state.envC, state.envE) state.store top
   ⇒
   ast_repl state (F::type_errors) (SOME ast::asts) Diverge) ∧
